Arithmetization.lean
@@ -22,4 +22,5 @@ import Arithmetization.ISigmaOne.HFS.Basic
 import Arithmetization.ISigmaOne.HFS.Seq
 import Arithmetization.ISigmaOne.HFS.PRF
 import Arithmetization.ISigmaOne.HFS.Supplemental
+import Arithmetization.ISigmaOne.HFS.Fixpoint
 import Arithmetization.ISigmaOne.Metamath.Term
